Hit a counter-example on le-completeness

MiniKernel/Proofs.lean
@@ -1,5 +1,19 @@
 import MiniKernel.Kernel
 
+@[grind] inductive Level.NF : Level → Prop
+  | zero : Level.NF .zero
+  | succ : Level.NF l → Level.NF (.succ l)
+  | max : Level.NF l1 → Level.NF l2 → Level.NF (.max l1 l2)
+  | imax : Level.NF l1 → Level.NF (.imax l1 (.param u))
+  | param : Level.NF (.param n)
+
+@[grind .] theorem Level.NF.mkIMax (h1 : Level.NF l1) (h2 : Level.NF l2) : Level.NF (.mkIMax l1 l2) := by
+  fun_induction Level.mkIMax <;> grind
+
+@[grind .] theorem Level.NF.simplify : Level.NF (simplify l) := by
+  fun_induction Level.simplify <;> grind
+
+
 def Level.eval (l : Level) (ctx : Name → Nat) : Nat :=
   match l with
   | .zero => 0
@@ -20,68 +34,197 @@ theorem Level.forall_zero_le_eval (balance : Int) (l : Level) :
     have := Level.eval_mono (fun _ => 0) ctx l (by grind)
     grind
 
-def Level.dependsOn (l : Level) (p : Name) : Prop :=
+def Option.imax (o1 o2 : Option Nat) : Option Nat :=
+  match o1, o2 with
+  | none, none => none
+  | _, none => none
+  | none, some n => some n
+  | some n1, some n2 => some (Nat.max n1 n2)
+
+def Level.coeff (l : Level) (p : Name) : Option Nat :=
   match l with
-  | .zero => False
-  | .succ l' => dependsOn l' p
-  | .max l1 l2 => dependsOn l1 p ∨ dependsOn l2 p
-  | .imax l1 l2 => dependsOn l1 p ∨ dependsOn l2 p
-  | .param n => n = p
+  | .zero => none
+  | .succ l' => .succ <$> coeff l' p
+  | .max l1 l2 => Max.max (coeff l1 p) (coeff l2 p)
+  | .imax l1 (.param n) => if n = p then Max.max (coeff l1 p) (some 0) else none
+  | .imax _ _ => none -- unreachable due to NF
+  | .param n => if n = p then some 0 else none
+
+theorem Level.coeff_le_eval_none (n : Nat) (l : Level) (p : Name)
+  (hwf : l.NF) (h : l.coeff p = none) : l.eval (fun p' => if p' = p then n else 0) = l.eval (fun _ => 0) := by
+  induction hwf generalizing n <;> simp_all only [coeff] <;> simp_all [eval]
+
+theorem Level.coeff_some_eval (l : Level) (p : Name) (hwf : l.NF) (h : l.coeff p = some c) :
+    ∃ n, ∀ m > n, l.eval (fun p' => if p' = p then m else 0) = c + m := by
+  induction hwf generalizing c <;> simp_all only [coeff, eval] <;> try grind [coeff, eval, Functor.map]
+  case succ l hwf ih =>
+    revert ih h; cases l.coeff p <;> intro ih h
+    · contradiction
+    · simp at h; subst c
+      obtain ⟨n, ih⟩ := ih rfl
+      exists n
+      intro m hm
+      grind
+  case max l1 l2 hwf1 hwf2 ih1 ih2 =>
+    revert ih1 ih2 h; cases hc1 : l1.coeff p <;> cases hc2 : l2.coeff p <;> intro ih1 ih2 h <;> simp at h
+    · subst c
+      clear ih1
+      obtain ⟨n2, ih2⟩ := ih2 rfl
+      exists Max.max (l1.eval (fun _ => 0)) n2
+      intro m hm
+      rw [Level.coeff_le_eval_none _ l1 p hwf1 hc1]
+      specialize ih2 m (by grind)
+      grind
+    · subst c
+      clear ih2
+      obtain ⟨n1, ih1⟩ := ih1 rfl
+      exists Max.max n1 (l2.eval (fun _ => 0))
+      intro m hm
+      rw [Level.coeff_le_eval_none _ l2 p hwf2 hc2]
+      specialize ih1 m (by grind)
+      grind
+    · subst c
+      obtain ⟨n1, ih1⟩ := ih1 rfl
+      obtain ⟨n2, ih2⟩ := ih2 rfl
+      exists Max.max n1 n2
+      intro m hm
+      specialize ih1 m (by grind)
+      specialize ih2 m (by grind)
+      grind
+  case imax l1 p' hwf1 ih1 =>
+    by_cases hp : p' = p
+    · simp [hp] at *
+      skip
+      revert ih1 h; cases h1 : l1.coeff p <;> intro ih1 h <;> simp at h <;> subst h
+      case pos.none =>
+        exists l1.eval (fun _ => 0)
+        intro m hm
+        rw [Level.coeff_le_eval_none _ l1 p hwf1 h1]
+        grind
+      case pos.some c =>
+        simp_all
+        obtain ⟨n1, ih1⟩ := ih1
+        exists n1
+        intro m hm
+        specialize ih1 m (by grind)
+        grind
+    · simp [hp] at *
+  case param n =>
+    simp at h
+    exists 0
+    grind
+
+theorem Level.coeff_le_eval_some (l : Level) (p : Name) (ctx : Name → Nat)
+  (hwf : l.NF) (h : l.coeff p = some n) (hp : 0 < ctx p) : n + ctx p ≤ l.eval ctx := by
+  induction hwf generalizing n <;> simp_all only [coeff] <;> try grind [coeff, eval, Functor.map]
+  case succ =>
+    simp_all [Functor.map, eval]; grind
+  case max l1 l2 hl1 hl2 ih1 ih2 =>
+    simp_all [eval]
+    revert ih1 ih2 h
+    cases l1.coeff p <;> cases l2.coeff p <;> grind
+  case imax l1 p' hl1 ih1 =>
+    simp_all [eval]
+    revert ih1 h
+    cases l1.coeff p <;> by_cases p' = p <;> grind
+
+theorem Level.forall_param_le_eval (balance : Int) (l : Level) (p : Name) (hwf : l.NF) :
+  (∀ ctx, ctx p ≤ l.eval ctx + balance) ↔
+  (0 ≤ l.eval (fun _ => 0) + balance ∧ ∃ n, l.coeff p = some n ∧ 0 ≤ n + balance) := by
+  cases h : l.coeff p
+  case none =>
+    constructor
+    · intro h
+      exfalso
+      specialize h (fun p' => if p' = p then Int.natAbs balance + l.eval (fun _ => 0) + 1 else 0)
+      have := Level.coeff_le_eval_none (Int.natAbs balance + l.eval (fun _ => 0) + 1) l p hwf ‹_›
+      simp_all
+      grind
+    · simp
+  case some n =>
+    constructor
+    · intro h
+      constructor
+      · apply h
+      · simp
+        obtain ⟨k, hk⟩ := Level.coeff_some_eval l p hwf ‹_›
+        specialize hk (k+1) (by grind)
+        specialize h (fun p' => if p' = p then k + 1 else 0)
+        rw [hk] at h; clear hk
+        grind
+    · intro ⟨h1,h2⟩ ctx
+      by_cases h0 : ctx p = 0
+      · simp [h0] at *
+        have := Level.eval_mono (fun _ => 0) ctx l (by grind)
+        grind
+      · have := Level.coeff_le_eval_some l p ctx hwf ‹_›
+        obtain ⟨_, heq, h2⟩ := h2
+        simp at heq; subst heq
+        grind
+
+theorem counter_example (p : Name) :
+  let l1 := Level.zero.succ
+  let l2 := .imax ((Level.param p).succ) (.param p)
+  let balance : Int := -1
+  let ctx1 := fun n => if n = p then 2 else 0
+  let ctx2 := fun n => if n = p then 0 else 0
+  (l1.NF) ∧ (l2.NF) ∧
+  (∀ ctx, ctx p ≤ (l1.max l2).eval ctx + balance) ∧
+  (¬ ctx1 p ≤ l1.eval ctx1 + balance) ∧ (¬ ctx2 p ≤ l2.eval ctx2 + balance) := by
+  constructor
+  · constructor; constructor
+  constructor
+  · constructor; constructor; constructor
+  constructor
+  · intro ctx
+    simp [Level.eval]
+    grind
+  · constructor
+    · simp [Level.eval]
+    · simp [Level.eval]
 
 /-
-theorem Level.param_le_eval_step (balance : Int) (l : Level) (p : Name)
-  (hd : l.dependsOn p)
-  (h1 : 1 ≤ l.eval (fun p' => if p' = p then 1 else 0) + balance) :
-  (∀ n, n + 1 ≤ l.eval (fun p' => if p' = p then n + 1 else 0) + balance) := by
-  intro n
-  induction l generalizing balance <;> simp [eval, dependsOn] at *
-  case succ ih =>
-    specialize ih (balance + 1) hd
-    grind
-  case max ih1 ih2 =>
-    simp [Int.le_max] at h1
-    cases hd
-    · specialize ih1 balance ‹_›
-
-      grind
-    · specialize ih2 balance ‹_›
-      grind
+theorem Level.forall_param_le_eval_max (balance : Int) (l1 l2 : Level) (p : Name)
+  (hwf1: l1.NF) (hwf2 : l2.NF) :
+   (∀ (ctx : Name → Nat), ↑(ctx p) ≤ ↑((l1.max l2).eval ctx) + balance) →
+   (∀ (ctx : Name → Nat), ↑(ctx p) ≤ ↑(l1.eval ctx) + balance) ∨ (∀ (ctx : Name → Nat), ↑(ctx p) ≤ ↑(l2.eval ctx) + balance) := by
+  simp [Level.forall_param_le_eval, hwf1, hwf2, NF.max, coeff]
+  simp [eval]
+  intro hle_max c hcoeff hle1
+  rw [Lean.Omega.Int.ofNat_max] at hle_max
+  rw [← Int.max_add_right] at hle_max
+  cases hc1 : l1.coeff p <;> cases hc2 : l2.coeff p <;> simp [hc1, hc2] at hcoeff
+  case none.some =>
+    subst hcoeff
 
 
-
-theorem Level.forall_param_le_eval (balance : Int) (l : Level) (p : Name) :
-  (∀ ctx, ctx p ≤ l.eval ctx + balance) ↔
-    (0 ≤ l.eval (fun _ => 0) + balance ∧ 1 ≤ l.eval (fun n => if n = p then 1 else 0) + balance)
-    := by
-  constructor
-  · intro h; constructor
-    · apply h
-    · specialize h (fun n => if n = p then 1 else 0)
-      grind
-  · intro ⟨h0, h1⟩ ctx
-    match h : ctx p with
-    | 0 =>
-      have := Level.eval_mono (fun _ => 0) ctx l (by grind)
-      simp_all
-      grind
-    | n+1 =>
-      have := Level.eval_mono (fun n' => if n' = p then 1 else 0) ctx l (by grind)
-      simp_all
-      grind
+  have hle_max : 0 ≤ (↑(l1.eval fun x => 0) + balance) ∨ 0 ≤ (↑(l2.eval fun x => 0) + balance) := by grind
+  cases hle_max <;> clear hle_max
+  case inl hl1 =>
+    left
+    constructor
+    · assumption
+    ·         constructor
+        ·
+        · grind
+      case some.none =>
 -/
+#exit
 
-@[grind] inductive Level.NF : Level → Prop
-  | zero : Level.NF .zero
-  | succ : Level.NF l → Level.NF (.succ l)
-  | max : Level.NF l1 → Level.NF l2 → Level.NF (.max l1 l2)
-  | imax : Level.NF l1 → Level.NF (.imax l1 (.param u))
-  | param : Level.NF (.param n)
 
-@[grind .] theorem Level.NF.mkIMax (h1 : Level.NF l1) (h2 : Level.NF l2) : Level.NF (.mkIMax l1 l2) := by
-  fun_induction Level.mkIMax <;> grind
 
-@[grind .] theorem Level.NF.simplify : Level.NF (simplify l) := by
-  fun_induction Level.simplify <;> grind
+theorem Level.forall_param_le_eval' (balance : Int) (l : Level) (p : Name) :
+  (∀ ctx, ctx p ≤ l.eval ctx + balance) ↔
+  (∀ n, n ≤ l.eval (fun n' => if n' = p then n else 0) + balance) := by
+  constructor
+  · intro h n
+    specialize h (fun n' => if n' = p then n else 0)
+    grind
+  · intro h ctx
+    specialize h (ctx p)
+    have := Level.eval_mono (fun n' => if n' = p then ctx p else 0) ctx l (by grind)
+    simp_all
+    grind
 
 @[grind =] theorem Level.mkIMax_correct (ctx : Name → Nat) (l1 l2 : Level): (mkIMax l1 l2).eval ctx = (Level.imax l1 l2).eval ctx := by
   fun_induction mkIMax<;> try grind [Level.eval]
@@ -197,7 +340,9 @@ theorem Level.le_complete (ctx : Name → Nat) (l1 l2 : Level) (balance : Int) :
   case case9 => -- param le max
     simp only [Bool.or_eq_true]
     simp [eval.eq_5] at *
-    -- simp [eval] at *
+    rw [Level.forall_param_le_eval] at *
+    simp [eval, coeff] at *
+    grind
     sorry
   case case10 => -- zero le max
     simp only [Bool.or_eq_true]
